end of day 02/04/19

inference-tool/src/main/scala/inference/Dirties.scala
@@ -111,31 +111,48 @@ object Dirties {
                             t1: Transition.transition_ext[Unit],
                             t2: Transition.transition_ext[Unit]): Boolean = {
                               if (HOL.equal(t1, t2)) {
-                                true
+                                return true
                               }
                               else if (Transition.Outputs(t1).length != Transition.Outputs(t2).length) {
-                                false
+                                return false
                               }
-                              else if (Code_Generation.all_literal_outputs(t1) &&
+                              println(f"Does\n${PrettyPrinter.transitionToString(t1)}\ndirectly subsume\n${PrettyPrinter.transitionToString(t2)}? y/n\n")
+                              if (Code_Generation.all_literal_outputs(t1) &&
                                        Code_Generation.all_literal_outputs(t2) &&
                                        Transition.Outputs(t1) != Transition.Outputs(t2)) {
-                                false
+                                println("n")
+                                return false
                               }
                               else if (Store_Reuse.is_proper_generalisation_of(t1, t2, b)) {
                                 // This needs modifying to model check but it should be OK for now
-                                println(f"Does\n${PrettyPrinter.transitionToString(t1)}\ndirectly subsume\n${PrettyPrinter.transitionToString(t2)}? y/n\n")
                                 println("y")
-                                true
+                                return true
                               }
                               else if (Store_Reuse.is_proper_generalisation_of(t2, t1, b)) {
                                 // This needs modifying to model check but it should be OK for now
-                                println(f"Does\n${PrettyPrinter.transitionToString(t1)}\ndirectly subsume\n${PrettyPrinter.transitionToString(t2)}? y/n\n")
                                 println("n")
-                                false
+                                return false
                               }
                               else {
-                                val subsumes = readLine(f"Does\n${PrettyPrinter.transitionToString(t1)}\ndirectly subsume\n${PrettyPrinter.transitionToString(t2)}? y/n\n") == "y"
+                                val subsumes = readLine("") == "y"
                                 subsumes
                               }
                             }
+
+    def scalaWeaklyDirectlySubsumes(e1: FSet.fset[(Nat.nat, ((Nat.nat, Nat.nat), Transition.transition_ext[Unit]))],
+                                    e2: FSet.fset[(Nat.nat, ((Nat.nat, Nat.nat), Transition.transition_ext[Unit]))],
+                                    s: Nat.nat,
+                                    s_prime: Nat.nat,
+                                    t1: Transition.transition_ext[Unit],
+                                    t2: Transition.transition_ext[Unit]): Boolean = {
+                                println(f"Does\n${PrettyPrinter.transitionToString(t1)}\nWEAKLY directly subsume\n${PrettyPrinter.transitionToString(t2)}? y/n\n")
+                                if (Increment_Reset.increment_inserted(t1, t2, e1, e2)) {
+                                  println("y")
+                                  true
+                                }
+                                else {
+                                  println("n")
+                                  false
+                                }
+                              }
   }
