formal/inference/heuristics/Increment_Reset.thy
@@ -1,5 +1,5 @@
 theory Increment_Reset
-  imports "../Inference"
+  imports "../Inference" "../Enable_Logging"
 begin
 
 definition initialiseReg :: "transition \<Rightarrow> vname \<Rightarrow> transition" where
@@ -17,9 +17,10 @@ fun insert_increment :: update_modifier where
           newReg = R r;
           newT1 = \<lparr>Label = Label t1, Arity = Arity t1, Guard = [], Outputs = [Plus (V newReg) (V (I 1))], Updates=((newReg, Plus (V newReg) (V (I 1)))#Updates t1)\<rparr>;
           newT2 = \<lparr>Label = Label t2, Arity = Arity t2, Guard = [], Outputs = [Plus (V newReg) (V (I 1))], Updates=((newReg, Plus (V newReg) (V (I 1)))#Updates t2)\<rparr>;
-          initialised = fimage (\<lambda>(uid, (from, to), t). (uid, (from, to), (if (to = dest t1ID new \<or> to = dest t2ID new) \<and> t \<noteq> t1 \<and> t \<noteq> t2 then initialiseReg t newReg else t))) new 
+          initialised = fimage (\<lambda>(uid, (from, to), t). (uid, (from, to), (if (to = dest t1ID new \<or> to = dest t2ID new) \<and> t \<noteq> t1 \<and> t \<noteq> t2 then initialiseReg t newReg else t))) new;
+          newEFSM = (replaceAll (replaceAll initialised t2 newT2) t1 newT1)
           in 
-          Some (replaceAll (replaceAll initialised t2 newT2) t1 newT1)
+          resolve_nondeterminism (sorted_list_of_fset (nondeterministic_pairs newEFSM)) old newEFSM null_modifier (\<lambda>a. True)
      else
        None
      )"
@@ -27,20 +28,50 @@ fun insert_increment :: update_modifier where
 definition struct_replace_all :: "iEFSM \<Rightarrow> transition \<Rightarrow> transition \<Rightarrow> iEFSM" where
   "struct_replace_all e old new = fimage (\<lambda>(uid, (from, dest), t). if same_structure t old then (uid, (from, dest), new) else (uid, (from, dest), t)) e"
 
+lemma output_match_symmetry: "(outputMatch t1 t2) = (outputMatch t2 t1)"
+  apply (simp add: outputMatch_def)
+  by auto
+
+lemma guard_match_symmetry: "(guardMatch t1 t2) = (guardMatch t2 t1)"
+  apply (simp add: guardMatch_def)
+  by auto
+
 fun insert_increment_2 :: update_modifier where
   "insert_increment_2 t1ID t2ID s new old = (let
      t1 = get_by_id new t1ID;
-     t2 = get_by_id new t2ID in
+     t2 = get_by_id new t2ID;
+     p = println (STR ''calling insert increment with '' + transition2string t1 + STR '' and ''+ transition2string t2);
+     p = println (STR ''guardMatch?''+ bool2string (guardMatch t1 t2));
+     p = println (STR ''outputMatch?''+ bool2string (outputMatch t1 t2)) in
+
      if guardMatch t1 t2 \<and> outputMatch t1 t2 then let 
+          p = println STR ''success'';
           r = max_reg new + 1;
           newReg = R r;
           newT1 = \<lparr>Label = Label t1, Arity = Arity t1, Guard = [], Outputs = [Plus (V newReg) (V (I 1))], Updates=((newReg, Plus (V newReg) (V (I 1)))#Updates t1)\<rparr>;
           newT2 = \<lparr>Label = Label t2, Arity = Arity t2, Guard = [], Outputs = [Plus (V newReg) (V (I 1))], Updates=((newReg, Plus (V newReg) (V (I 1)))#Updates t2)\<rparr>;
-          initialised = fimage (\<lambda>(uid, (from, to), t). (uid, (from, to), (if (to = dest t1ID new \<or> to = dest t2ID new) \<and> t \<noteq> t1 \<and> t \<noteq> t2 then initialiseReg t newReg else t))) new 
+          initialised = fimage (\<lambda>(uid, (from, to), t). (uid, (from, to), (if (to = dest t1ID new \<or> to = dest t2ID new) \<and> t \<noteq> t1 \<and> t \<noteq> t2 then initialiseReg t newReg else t))) new ;
+          newEFSM = (struct_replace_all (struct_replace_all initialised t2 newT2) t1 newT1);
+          p = writeiDot newEFSM (STR ''dotfiles/log/''+timestamp+STR ''.dot'')
           in 
-          Some (struct_replace_all (struct_replace_all initialised t2 newT2) t1 newT1)
+          resolve_nondeterminism (sorted_list_of_fset (nondeterministic_pairs newEFSM)) old newEFSM null_modifier (\<lambda>a. True)
      else
+       let p = println STR ''failure'' in
        None
      )"
+
+fun guardMatch_alt_2 :: "gexp list \<Rightarrow> bool" where
+  "guardMatch_alt_2 [(gexp.Eq (V (I i)) (L (Num n)))] = (i = 1)" |
+  "guardMatch_alt_2 _ = False"
+
+fun outputMatch_alt_2 :: "aexp list \<Rightarrow> bool" where
+  "outputMatch_alt_2 [(L (Num n))] = True" |
+  "outputMatch_alt_2 _ = False"
+
+definition increment_inserted :: "transition \<Rightarrow> transition \<Rightarrow> iEFSM \<Rightarrow> iEFSM \<Rightarrow> bool" where
+  "increment_inserted t1 t2 e1 e2 \<equiv> guardMatch_alt_2 (Guard t1) \<and>
+                                    outputMatch_alt_2 (Outputs t1) \<and>
+                                    Updates t1 =[] \<and>
+                                    (\<exists>r \<in> (all_regs e2 - all_regs e1). t2 = \<lparr>Label = Label t1, Arity = Arity t1, Guard = [], Outputs = [Plus (V (R r)) (V (I 1))], Updates=(((R r), Plus (V (R r)) (V (I 1)))#Updates t1)\<rparr>)"
 
 end
